doc/formalization/Catala.Translation.Helpers.fst
@@ -1,0 +1,625 @@
+module Catala.Translation.Helpers
+
+open Catala.LambdaCalculus
+
+(*** Default translation *)
+
+let process_exceptions_f (tau: ty) : Tot exp =
+  EAbs (TOption tau) (EAbs (TArrow TUnit tau) (
+    EApp (EAbs (TOption tau) (
+      EMatchOption (EVar 2) tau
+        (EVar 0)
+        (EAbs tau (
+          EMatchOption (EVar 1) tau
+            (EVar 3)
+            (EAbs tau (ELit (LError ConflictError)))
+        ))
+    ))
+    (ECatchEmptyError (ESome (EApp (EVar 0) (ELit LUnit) TUnit)) ENone)
+    (TOption tau)
+  ))
+
+let typ_process_exceptions_f (g: env) (tau: ty)
+    : Lemma (typing g (process_exceptions_f tau)
+      (TArrow (TOption tau) (TArrow (TArrow TUnit tau) (TOption tau))))
+  =
+  assert_norm(typing g (process_exceptions_f tau)
+      (TArrow (TOption tau) (TArrow (TArrow TUnit tau) (TOption tau))))
+
+let build_default_translation
+  (exceptions: list exp)
+  (acc: exp)
+  (just: exp)
+  (cons: exp)
+  (tau: ty)
+  =
+  EMatchOption
+    (EFoldLeft
+      (process_exceptions_f tau)
+      acc (TOption tau)
+      (EList exceptions) (TArrow TUnit tau))
+    tau
+    (EIf
+      just cons
+      (ELit (LError EmptyError)))
+    (EAbs tau (EVar 0))
+
+#push-options "--fuel 1 --ifuel 0"
+let build_default_translation_typing
+  (exceptions: list exp)
+  (acc: exp)
+  (just: exp)
+  (cons: exp)
+  (tau: ty)
+  (g: env)
+    : Lemma
+      (requires (
+        typing_list g exceptions (TArrow TUnit tau) /\
+        typing g acc (TOption tau) /\
+        typing g just TBool /\
+        typing g cons tau))
+      (ensures (typing g (build_default_translation exceptions acc just cons tau) tau))
+  =
+  typ_process_exceptions_f g tau;
+  assert_norm(typing g (build_default_translation exceptions acc just cons tau) tau)
+#pop-options
+
+#push-options "--fuel 9 --ifuel 0"
+let process_exceptions_untouched_by_subst (s: var_to_exp) (tau: ty) : Lemma
+    (subst s (process_exceptions_f tau) == process_exceptions_f tau)
+  =
+  ()
+#pop-options
+
+(*** Step lifting framework *)
+
+let typed_l_exp (tau: ty) = e:exp{typing empty e tau}
+
+let rec take_l_steps (tau: ty) (e: typed_l_exp tau) (fuel: nat)
+    : Tot (option (typed_l_exp tau))
+      (decreases fuel) =
+  if fuel = 0 then Some e else
+  match step e with
+  | None -> None
+  | Some e' ->
+    preservation e tau;
+    take_l_steps tau e' (fuel - 1)
+
+#push-options "--fuel 2 --ifuel 1"
+let rec take_l_steps_transitive (tau: ty) (e1 e2: typed_l_exp tau) (n1 n2: nat)
+    : Lemma
+      (requires (take_l_steps tau e1 n1 == Some e2))
+      (ensures (take_l_steps tau e1 (n1 + n2) == take_l_steps tau e2 n2))
+      (decreases n1)
+  =
+  if n1 = 0 then () else begin
+    match step e1 with
+      | None -> ()
+      | Some e1' ->
+        preservation e1 tau;
+        take_l_steps_transitive tau e1' e2 (n1 - 1) n2
+  end
+#pop-options
+
+let not_l_value (tau: ty) = e:exp{not (is_value e) /\ typing empty e tau}
+let l_value (tau: ty) = e:exp{is_value e /\ typing empty e tau}
+
+let stepping_context (tau tau': ty) = typed_l_exp tau -> not_l_value tau'
+
+let step_lift_commute_non_value
+  (tau tau': ty)
+  (f: stepping_context tau tau')
+  (e: typed_l_exp tau)
+    : prop
+  =
+  progress e tau;
+  if is_value e then true else begin
+    preservation e tau;
+    step (f e) == Some (f (Some?.v (step e)))
+  end
+
+let is_stepping_agnostic_lift
+  (tau tau': ty)
+  (f:stepping_context tau tau')
+    : prop
+  =
+  forall (e: typed_l_exp tau). step_lift_commute_non_value tau tau' f e
+
+let stepping_agnostic_lift
+  (tau tau': ty)
+  : Type
+  = f:(stepping_context tau tau'){is_stepping_agnostic_lift tau tau' f}
+
+let rec l_values_dont_step (e: exp) : Lemma
+    (requires (is_value e))
+    (ensures (step e = None))
+    (decreases %[e; 1])
+  =
+  match e with
+  | EAbs _ _ -> ()
+  | EThunk _ -> ()
+  | ELit _ -> ()
+  | ENone -> ()
+  | EList [] -> ()
+  | EList l -> l_values_dont_step_list e l
+  | _ -> ()
+and l_values_dont_step_list (e: exp) (l: list exp{l << e /\ Cons? l}) : Lemma
+    (requires (is_value_list l))
+    (ensures (step_list e l = Bad))
+    (decreases %[e; 0; l])
+  =
+  match l with
+  | [hd] -> l_values_dont_step hd
+  | hd::tl ->
+    l_values_dont_step hd;
+    l_values_dont_step_list e tl
+
+#push-options "--z3rlimit 50 --fuel 2 --ifuel 1"
+let rec lift_multiple_l_steps
+  (tau tau': ty)
+  (e1: typed_l_exp tau)
+  (e2: typed_l_exp tau)
+  (n: nat)
+  (f : stepping_agnostic_lift tau tau')
+    : Lemma
+      (requires (take_l_steps tau e1 n == Some e2))
+      (ensures (take_l_steps tau' (f e1) n == Some (f e2)))
+      (decreases n)
+  =
+  match step e1 with
+  | None -> ()
+  | Some e1' ->
+    progress e1 tau;
+    preservation e1 tau;
+    if is_value e1 then
+      l_values_dont_step e1
+    else if n = 0 then
+      ()
+    else
+      lift_multiple_l_steps tau tau' e1' e2 (n-1) f
+#pop-options
+
+
+(*** Lifts *)
+
+let if_cond_lift'
+  (tau: ty)
+  (e2 e3: typed_l_exp tau)
+    : stepping_context TBool tau
+  =
+  fun e1 -> EIf e1 e2 e3
+
+let if_cond_lift_is_stepping_agnostic
+  (tau: ty)
+  (e2 e3: typed_l_exp tau)
+  (e: typed_l_exp TBool)
+    : Lemma
+      (requires (True))
+      (ensures (step_lift_commute_non_value TBool tau (if_cond_lift' tau e2 e3) e))
+  =
+  progress e TBool; if is_value e then () else preservation e TBool
+
+let if_cond_lift
+  (tau: ty)
+  (e2 e3: typed_l_exp tau)
+    : stepping_agnostic_lift TBool tau
+  =
+  Classical.forall_intro (if_cond_lift_is_stepping_agnostic tau e2 e3);
+  if_cond_lift' tau e2 e3
+
+
+let app_f_lift'
+  (tau_arg tau: ty)
+  (e2: typed_l_exp tau_arg)
+    : stepping_context (TArrow tau_arg tau) tau
+  =
+  fun e1 -> EApp e1 e2 tau_arg
+
+let app_f_lift_is_stepping_agnostic
+  (tau_arg tau: ty)
+  (e2: typed_l_exp tau_arg)
+  (e: typed_l_exp (TArrow tau_arg tau))
+    : Lemma
+      (requires (True))
+      (ensures (
+        step_lift_commute_non_value (TArrow tau_arg tau) tau (app_f_lift' tau_arg tau e2) e))
+  =
+  progress e  (TArrow tau_arg tau);
+  if is_value e then () else preservation e  (TArrow tau_arg tau)
+
+let app_f_lift
+  (tau_arg tau: ty)
+  (e2: typed_l_exp tau_arg)
+    : stepping_agnostic_lift (TArrow tau_arg tau) tau
+  =
+  Classical.forall_intro (app_f_lift_is_stepping_agnostic tau_arg tau e2);
+  app_f_lift' tau_arg tau e2
+
+let app_arg_lift'
+  (tau_arg tau: ty)
+  (e1: l_value (TArrow tau_arg tau))
+    : stepping_context tau_arg tau
+  =
+  fun e2 -> EApp e1 e2 tau_arg
+
+let app_arg_lift_is_stepping_agnostic
+  (tau_arg tau: ty)
+  (e1: l_value (TArrow tau_arg tau){match e1 with ELit (LError _) -> False | _ -> True})
+  (e2: typed_l_exp tau_arg)
+    : Lemma
+      (requires (True))
+      (ensures (
+        step_lift_commute_non_value tau_arg tau (app_arg_lift' tau_arg tau e1) e2))
+  =
+  progress e2 tau_arg;
+  if is_value e2 then () else preservation e2 tau_arg
+
+let app_arg_lift
+  (tau_arg tau: ty)
+  (e1: l_value (TArrow tau_arg tau){match e1 with ELit (LError _) -> False | _ -> True})
+    : stepping_agnostic_lift tau_arg tau
+  =
+  Classical.forall_intro (app_arg_lift_is_stepping_agnostic tau_arg tau e1);
+  app_arg_lift' tau_arg tau e1
+
+#push-options "--fuel 9 --ifuel 2 --z3rlimit 30"
+let exceptions_head_lift'
+  (tau: ty)
+  (tl: list exp{typing_list empty tl (TArrow TUnit tau)})
+  (acc: typed_l_exp (TOption tau))
+  (just: (typed_l_exp TBool))
+  (cons: (typed_l_exp tau))
+  : stepping_context tau tau
+  =
+  fun (hd: typed_l_exp tau) ->
+    typ_process_exceptions_f empty tau;
+    typing_empty_can_be_extended acc (TOption tau) (extend empty (TOption tau));
+    typing_empty_can_be_extended acc (TOption tau)
+    (extend (extend empty (TOption tau)) tau);
+    EMatchOption
+    (EFoldLeft
+      (process_exceptions_f tau)
+      (EApp
+        (EAbs (TOption tau) (
+          EMatchOption acc tau
+            (EVar 0)
+            (EAbs tau (
+              EMatchOption (EVar 1) tau
+                acc
+                (EAbs tau (ELit (LError ConflictError)))
+            ))
+         ))
+         (ECatchEmptyError
+           (ESome hd) ENone)
+         (TOption tau)
+      )
+      (TOption tau)
+      (EList tl) (TArrow TUnit tau))
+    tau
+    (EIf
+      just cons
+      (ELit (LError EmptyError)))
+    (EAbs tau (EVar 0))
+#pop-options
+
+let exceptions_head_lift_is_stepping_agnostic
+  (tau: ty)
+  (tl: list exp{typing_list empty tl (TArrow TUnit tau)})
+  (acc: typed_l_exp (TOption tau))
+  (just: (typed_l_exp TBool))
+  (cons: (typed_l_exp tau))
+  (hd: typed_l_exp tau)
+    : Lemma (step_lift_commute_non_value tau tau (exceptions_head_lift' tau tl acc just cons) hd)
+  =
+  progress hd tau;
+  if is_value hd then () else begin
+    preservation hd tau;
+    assert_norm(step (exceptions_head_lift' tau tl acc just cons hd) == Some
+      (exceptions_head_lift' tau tl acc just cons (Some?.v (step hd))))
+  end
+
+let exceptions_head_lift
+  (tau: ty)
+  (tl: list exp{typing_list empty tl (TArrow TUnit tau)})
+  (acc: typed_l_exp (TOption tau))
+  (just: (typed_l_exp TBool))
+  (cons: (typed_l_exp tau))
+  : stepping_agnostic_lift tau tau
+  =
+  Classical.forall_intro (exceptions_head_lift_is_stepping_agnostic tau tl acc just cons);
+  exceptions_head_lift' tau tl acc just cons
+
+#push-options "--fuel 3 --ifuel 0"
+let exceptions_init_lift'
+  (tau: ty)
+  (tl: list exp{typing_list empty tl (TArrow TUnit tau)})
+  (just: (typed_l_exp TBool))
+  (cons: (typed_l_exp tau))
+  : stepping_context (TOption tau) tau
+  =
+  fun (init: typed_l_exp (TOption tau)) ->
+    typ_process_exceptions_f empty tau;
+    EMatchOption
+    (EFoldLeft
+      (process_exceptions_f tau)
+      init
+      (TOption tau)
+      (EList tl) (TArrow TUnit tau))
+    tau
+    (EIf
+      just cons
+      (ELit (LError EmptyError)))
+    (EAbs tau (EVar 0))
+#pop-options
+
+let exceptions_init_lift_is_stepping_agnostic
+  (tau: ty)
+  (tl: list exp{typing_list empty tl (TArrow TUnit tau)})
+  (just: (typed_l_exp TBool))
+  (cons: (typed_l_exp tau))
+  (init: typed_l_exp (TOption tau))
+    : Lemma (
+      step_lift_commute_non_value (TOption tau) tau (exceptions_init_lift' tau tl just cons) init)
+  =
+  progress init (TOption tau);
+  if is_value init then () else begin
+    preservation init (TOption tau);
+    assert_norm(step (exceptions_init_lift' tau tl just cons init) == Some
+      (exceptions_init_lift' tau tl just cons (Some?.v (step init))))
+  end
+
+let exceptions_init_lift
+  (tau: ty)
+  (tl: list exp{typing_list empty tl (TArrow TUnit tau)})
+  (just: (typed_l_exp TBool))
+  (cons: (typed_l_exp tau))
+  : stepping_agnostic_lift (TOption tau) tau
+  =
+  Classical.forall_intro (exceptions_init_lift_is_stepping_agnostic tau tl just cons);
+  exceptions_init_lift' tau tl just cons
+
+
+#push-options "--fuel 7 --ifuel 2 --z3rlimit 50"
+let lift_multiple_l_steps_exceptions_head
+  (tau: ty)
+  (tl: list exp{typing_list empty tl (TArrow TUnit tau) /\ is_value_list tl})
+  (acc: typed_l_exp (TOption tau))
+  (just: (typed_l_exp TBool))
+  (cons: (typed_l_exp tau))
+  (n_hd: nat)
+  (hd: typed_l_exp tau)
+  (final_hd: typed_l_exp tau)
+    : Lemma
+      (requires (take_l_steps tau hd n_hd == Some final_hd /\ is_value acc))
+      (ensures (
+        build_default_translation_typing
+          ((EThunk hd)::tl) acc just cons tau empty;
+        take_l_steps tau
+          (build_default_translation ((EThunk hd)::tl) acc just cons tau)
+          (n_hd + 4) ==
+            Some (exceptions_head_lift tau tl acc just cons final_hd)))
+  =
+  build_default_translation_typing ((EThunk hd)::tl) acc just cons tau empty;
+  typing_empty_can_be_extended acc (TOption tau) (extend empty (TOption tau));
+  typing_empty_can_be_extended acc (TOption tau)
+   (extend (extend empty (TOption tau)) tau);
+  let init_stepped : typed_l_exp (TOption tau) = EApp (EAbs (TOption tau) (
+    EMatchOption acc tau (EVar 0) (EAbs tau (
+      EMatchOption (EVar 1) tau acc (EAbs tau
+        (ELit (LError ConflictError))
+      )
+    ))))
+    (ECatchEmptyError (ESome hd) ENone) (TOption tau)
+  in
+  let init = EApp
+    (EApp (process_exceptions_f tau) acc (TOption tau))
+    (EThunk hd) (TArrow TUnit tau)
+  in
+  let open FStar.Tactics in
+  assert(take_l_steps (TOption tau) init 3 == Some init_stepped) by begin
+    compute ();
+    tadmit ()
+  end;
+  let default_translation: typed_l_exp tau =
+    build_default_translation ((EThunk hd)::tl) acc just cons tau
+  in
+  let default_translation_stepped = EMatchOption
+    (EFoldLeft
+      (process_exceptions_f tau)
+      init (TOption tau)
+      (EList tl) (TArrow TUnit tau))
+    tau
+    (EIf
+      just cons
+      (ELit (LError EmptyError)))
+    (EAbs tau (EVar 0))
+  in
+  assert(take_l_steps tau default_translation 1 == Some default_translation_stepped);
+  admit();
+  assert(default_translation_stepped == exceptions_init_lift tau tl just cons
+    (EApp (EApp (process_exceptions_f tau) ENone (TOption tau))
+      (EThunk hd) (TArrow TUnit tau)));
+  lift_multiple_l_steps (TOption tau) tau init init_stepped 3
+    (exceptions_init_lift tau tl just cons);
+  assert(take_l_steps tau default_translation_stepped 3 ==
+    Some (exceptions_head_lift tau tl acc just cons hd));
+  take_l_steps_transitive tau default_translation default_translation_stepped 1 3;
+  assert(take_l_steps tau default_translation 4 ==
+    Some (exceptions_head_lift tau tl acc just cons hd));
+  lift_multiple_l_steps tau tau hd final_hd n_hd (exceptions_head_lift tau tl acc just cons);
+  assert(take_l_steps tau (exceptions_head_lift tau tl acc just cons hd) n_hd ==
+    Some (exceptions_head_lift tau tl acc just cons final_hd));
+  take_l_steps_transitive tau default_translation
+    (exceptions_head_lift tau tl acc just cons hd) 4 n_hd
+#pop-options
+
+(*** Various lambda calculus steps *)
+
+
+let process_exceptions_applied
+  (tau: ty)
+  (acc: typed_l_exp (TOption tau))
+  (hd: typed_l_exp tau)
+    : Tot (typed_l_exp (TOption tau))
+  =
+  typ_process_exceptions_f empty tau;
+  typing_empty_can_be_extended hd tau (extend empty TUnit);
+  EApp
+   (EApp (process_exceptions_f tau) acc (TOption tau))
+   (EThunk hd) (TArrow TUnit tau)
+
+
+#push-options "--fuel 7 --ifuel 2"
+let process_exceptions_applied_stepped
+  (tau: ty)
+  (acc: typed_l_exp (TOption tau))
+  (hd: typed_l_exp tau)
+    : Tot (typed_l_exp (TOption tau))
+  =
+  typing_empty_can_be_extended acc (TOption tau) (extend empty (TOption tau));
+  typing_empty_can_be_extended acc (TOption tau)
+   (extend (extend empty (TOption tau)) tau);
+  EApp (EAbs (TOption tau) (
+    EMatchOption acc tau (EVar 0) (EAbs tau (
+      EMatchOption (EVar 1) tau acc (EAbs  tau
+        (ELit (LError ConflictError))
+      )
+    ))))
+    (ECatchEmptyError (ESome hd) ENone) (TOption tau)
+#pop-options
+
+#push-options "--fuel 8 --ifuel 1 --z3rlimit 50"
+let process_exceptions_applied_stepping
+  (tau: ty)
+  (acc: typed_l_exp (TOption tau){is_value acc /\ not (is_error acc)})
+  (hd: typed_l_exp tau)
+    : Lemma (take_l_steps (TOption tau) (process_exceptions_applied tau acc hd) 3 ==
+      Some (process_exceptions_applied_stepped tau acc hd))
+  =
+  let e1 : exp =
+    EApp
+      (EAbs (TArrow TUnit tau) (
+    EApp (EAbs (TOption tau) (
+      EMatchOption acc tau
+        (EVar 0)
+        (EAbs  tau (
+          EMatchOption (EVar 1) tau
+            acc
+            (EAbs tau (ELit (LError ConflictError)))
+        ))
+    ))
+    (ECatchEmptyError (ESome (EApp (EVar 0) (ELit LUnit) TUnit)) ENone)
+    (TOption tau)
+  )
+      )
+      (EThunk hd) (TArrow TUnit tau)
+  in
+  let e2 =
+    EApp (EAbs (TOption tau) (
+      EMatchOption acc tau
+        (EVar 0)
+        (EAbs tau (
+          EMatchOption (EVar 1) tau
+            acc
+            (EAbs tau (ELit (LError ConflictError)))
+        ))
+    ))
+    (ECatchEmptyError (ESome (EApp (EThunk hd) (ELit LUnit) TUnit)) ENone)
+    (TOption tau)
+
+  in
+  assume(forall (s: var_to_exp). {:pattern (subst s acc) } subst s acc == acc);
+  assume(forall (s: var_to_exp). {:pattern (subst s (EThunk hd)) } subst s (EThunk hd) == (EThunk hd));
+  assert_norm(step (process_exceptions_applied tau acc hd) == Some e1);
+  assume(step e1 == Some e2);
+  let e3 =
+    EApp (EAbs (TOption tau) (
+      EMatchOption acc tau
+        (EVar 0)
+        (EAbs tau (
+          EMatchOption (EVar 1) tau
+            acc
+            (EAbs tau (ELit (LError ConflictError)))
+        ))
+    ))
+    (ECatchEmptyError (ESome hd) ENone)
+    (TOption tau)
+  in
+  assert_norm(step e2 == Some e3);
+  // Mostly proven?
+  admit()
+#pop-options
+
+#push-options "--fuel 2 --ifuel 1 --z3rlimit 40"
+let exceptions_head_lift_steps_to_error
+  (tau: ty)
+  (tl: list exp{is_value_list tl /\ typing_list empty tl (TArrow TUnit tau)})
+  (acc: typed_l_exp (TOption tau){is_value acc})
+  (just: (typed_l_exp TBool))
+  (cons: (typed_l_exp tau))
+    : Lemma (take_l_steps tau
+      (exceptions_head_lift tau tl acc just cons (ELit (LError ConflictError))) 5 ==
+        Some (ELit (LError ConflictError)))
+  =
+  let e = exceptions_head_lift tau tl acc just cons (ELit (LError ConflictError)) in
+  let e_plus_3 : typed_l_exp tau =
+    exceptions_init_lift tau tl just cons (ELit (LError ConflictError))
+  in
+  let open FStar.Tactics in
+  assert(take_l_steps tau e 3 == Some e_plus_3) by begin
+    compute ();
+    smt ()
+  end;
+  let e_plus_4 : typed_l_exp tau = EMatchOption
+    (ELit (LError ConflictError))
+    tau
+    (EIf
+      just cons
+      (ELit (LError EmptyError)))
+    (EAbs tau (EVar 0))
+  in
+  assert(step e_plus_3 == Some e_plus_4) by begin
+    compute ();
+    smt ()
+  end;
+  preservation e_plus_3 tau;
+  assert(Some e_plus_4 == take_l_steps tau e_plus_3 1);
+  assert(step e_plus_4 ==  Some (ELit (LError ConflictError)));
+  assert(take_l_steps tau e_plus_4 1 == Some (ELit (LError ConflictError)));
+  take_l_steps_transitive tau e e_plus_3 3 1;
+  take_l_steps_transitive tau e e_plus_4 4 1
+#pop-options
+
+
+let step_exceptions_head_value
+  (tau: ty)
+  (tl: list exp{is_value_list tl /\ typing_list empty tl (TArrow TUnit tau)})
+  (acc: (typed_l_exp (TOption tau)))
+  (just: (typed_l_exp TBool))
+  (cons: (typed_l_exp tau))
+  (hd: (typed_l_exp tau))
+    : Pure (typed_l_exp (TOption tau) & nat)
+      (requires (True))
+      (ensures (fun (new_acc, n) ->
+        is_value new_acc /\
+        take_l_steps tau (exceptions_head_lift tau tl acc just cons hd) n ==
+          Some (exceptions_init_lift tau tl just cons new_acc)
+      ))
+  =
+  admit()
+
+let step_exceptions_head_value_same_acc_result
+  (tau: ty)
+  (tl: list exp{is_value_list tl /\ typing_list empty tl (TArrow TUnit tau)})
+  (tl': list exp{is_value_list tl' /\ typing_list empty tl' (TArrow TUnit tau)})
+  (acc: (typed_l_exp (TOption tau)))
+  (just: (typed_l_exp TBool))
+  (cons: (typed_l_exp tau))
+  (hd: (typed_l_exp tau))
+    : Lemma (
+      let new_acc, _ = step_exceptions_head_value tau tl acc just cons hd in
+      let new_acc', _ = step_exceptions_head_value tau tl' acc just cons hd in
+      new_acc == new_acc'
+    )
+  =
+  admit()
